Clap/Lang/All.lean
@@ -1,0 +1,4 @@
+import Clap.Lang.F.F
+import Clap.Lang.FB.assert
+import Clap.Lang.FB.FB
+import Clap.Lang.FB.not
