Clap/eDSLState/Exp.lean
@@ -1,0 +1,61 @@
+import Clap.Circuit
+
+import Clap.eDSLState.Wheels
+
+namespace Clap
+
+abbrev FixedExp (p : ℕ) := Clap.Exp p ℕ
+abbrev FixedCircuit (p : ℕ) := Clap.Circuit p ℕ
+
+def FixedExp.eval {p : ℕ} (varStore : ℕ → Option (ZMod p)) (x : FixedExp p) : Option (ZMod p) :=
+  match x with
+  | .c x => .some x
+  | .v x => varStore x
+  | .add l r => do (←eval varStore l) + (←eval varStore r)
+  | .sub l r => do (←eval varStore l) - (←eval varStore r)
+  | .mul l r => do (←eval varStore l) * (←eval varStore r)
+
+@[simp, grind =]
+lemma eval_const
+  {p : ℕ}
+  {k : ZMod p}
+  {varStore : ℕ → Option (ZMod p)}
+:
+  FixedExp.eval varStore (Exp.c k) = .some k
+:= by
+  simp [FixedExp.eval]
+
+@[simp, grind =]
+lemma FixedExp.eval_add
+  {p : ℕ}
+  {varStore : ℕ → Option (ZMod p)}
+  {a b : FixedExp p}
+:
+  FixedExp.eval varStore (a + b) =
+  FixedExp.eval varStore (Exp.add a b)
+:= by
+  simp [HAdd.hAdd, Add.add]
+
+@[simp, grind =]
+lemma FixedExp.eval_sub
+  {p : ℕ}
+  {varStore : ℕ → Option (ZMod p)}
+  {a b : FixedExp p}
+:
+  FixedExp.eval varStore (a - b) =
+  FixedExp.eval varStore (Exp.sub a b)
+:= by
+  simp [HSub.hSub, Sub.sub]
+
+@[simp, grind =]
+lemma FixedExp.eval_mul
+  {p : ℕ}
+  {varStore : ℕ → Option (ZMod p)}
+  {a b : FixedExp p}
+:
+  FixedExp.eval varStore (a * b) =
+  FixedExp.eval varStore (Exp.mul a b)
+:= by
+  simp [HMul.hMul, Mul.mul]
+
+end Clap
