Clap/eDSLState/Monad.lean
@@ -1,0 +1,138 @@
+import Mathlib.Control.Monad.Writer
+
+import Clap.eDSLState.Circuit
+
+namespace Clap
+
+namespace Edsl
+
+variable {p : ℕ}
+
+abbrev CircuitStateM (p : ℕ) (α : Type) : Type := WriterT (CircuitState p) (StateM ℕ) α
+
+-- TODO do we really want this instance, or do we create it locally in order to create LawfulMonad manually?
+instance (p : ℕ) : Monoid (CircuitState p) where
+  mul := Array.append
+  mul_assoc := by apply Array.append_assoc
+  one := #[]
+  one_mul := by apply Array.empty_append
+  mul_one := by apply Array.append_empty
+
+@[simp, grind =]
+lemma CircuitState.mul_eq_append (a b: CircuitState p) :
+  a * b = a ++ b
+:= rfl
+
+@[simp, grind =]
+lemma CircuitState.one_eq_empty :
+  (1: CircuitState p) = #[]
+:= rfl
+
+#synth LawfulMonad (CircuitStateM 57)
+
+def CircuitStateM.run {p : ℕ} {α : Type} (cmd : CircuitStateM p α) (numAlloc : ℕ) :=
+  StateT.run (WriterT.run cmd) numAlloc
+
+attribute [Clap.monads]
+  bind
+  pure
+
+  CircuitStateM.run
+
+  WriterT.run
+  WriterT.mk
+  tell
+
+  StateT.run
+  StateT.bind
+  StateT.pure
+  StateT.map
+
+  Functor.map
+
+attribute [local implicit_reducible]
+  StateT
+  WriterT
+  Id
+
+def CircuitStateM.alloc {p : ℕ} : CircuitStateM p ℕ:=
+  getModify (· + 1)
+
+namespace CircuitState
+
+@[simp, grind =]
+lemma eval_bind
+  {α β : Type}
+  {varStore : Std.ExtTreeMap ℕ (ZMod p)}
+  {numAlloc : ℕ}
+  {action : CircuitStateM p α}
+  {function : α → CircuitStateM p β}
+:
+  eval (CircuitStateM.run (action >>= function) numAlloc).1.2 varStore numAlloc =
+  let ((result, action_circuit), numAlloc') := action.run numAlloc
+  let ((_, function_circuit), _) := (function result).run numAlloc'
+  let first_eval := eval action_circuit varStore numAlloc
+  let second_eval := eval function_circuit first_eval.varStore first_eval.numAlloc
+  {
+    numAlloc := second_eval.numAlloc
+    varStore := second_eval.varStore
+    constraints := first_eval.constraints ∧ second_eval.constraints
+  }
+:= by
+  simp only [Clap.monads]
+  grind
+
+end CircuitState
+
+namespace CircuitStateM
+
+@[Clap.monads]
+lemma getModify_eq
+  (numAlloc : ℕ) (f : ℕ → ℕ)
+:
+  @getModify
+    ℕ
+    (CircuitStateM p)
+    (instMonadStateOfMonadStateOf ℕ (CircuitStateM p))
+    f
+    numAlloc =
+    ((numAlloc, #[]), f numAlloc)
+:= rfl
+
+@[simp, grind =]
+lemma alloc_eq
+  (numAlloc : ℕ)
+:
+  CircuitStateM.alloc (p := p) numAlloc =
+  ((numAlloc, #[]), numAlloc + 1)
+:= by
+  simp [CircuitStateM.alloc, Clap.monads]
+
+-- TODO should this be in just simp, and/or grind?
+@[Clap.monads]
+lemma Vector_ofFnM_empty_state
+  (α)
+  (n)
+  (a : Fin n → ℕ → α)
+  (c : Fin n → ℕ → ℕ)
+  (numAlloc: ℕ)
+:
+  (@Vector.ofFnM (CircuitStateM p) _ n _ (λ x s => ⟨⟨a x s, #[]⟩, c x s⟩) numAlloc).1.2 =
+  #[]
+:= by
+  induction n with
+  | zero =>
+    simp [Vector.ofFnM_zero, Clap.monads]
+  | succ n h =>
+    rewrite [Vector.ofFnM_succ]
+    simp_all [Clap.monads]
+    set x := @Vector.ofFnM (CircuitStateM p) _ _ _ _ _
+    have : x = ⟨x.1, x.2⟩ := rfl
+    rewrite [this]; clear this
+    simp [x, h]
+
+end CircuitStateM
+
+end Edsl
+
+end Clap
