Clap/eDSLState/eDSL.lean
@@ -1,0 +1,163 @@
+import Clap.eDSLState.Monad
+
+namespace Clap.Edsl
+
+variable {p : ℕ}
+
+-- TODO split this into a file
+@[irreducible]
+def eq0 (e : FixedExp p) : CircuitStateM p Unit := do
+  tell #[.eq0 e]
+
+@[irreducible]
+def lam : CircuitStateM p (FixedExp p) := do
+  tell #[.lam]
+  let numAlloc ← CircuitStateM.alloc
+  return .v numAlloc
+
+@[irreducible]
+def share (e : FixedExp p) : CircuitStateM p (FixedExp p) := do
+  tell #[.share e]
+  let numAlloc ← CircuitStateM.alloc
+  return (.v numAlloc)
+
+@[irreducible]
+def isZero (e : FixedExp p) : CircuitStateM p (FixedExp p) := do
+  tell #[.isZero e]
+  let numAlloc ← CircuitStateM.alloc -- (un)just one
+  return .v numAlloc
+
+@[irreducible]
+def num2bits (width : ℕ) (e : FixedExp p) : CircuitStateM p (Vector (FixedExp p) width) := do
+  tell #[.num2bits width e]
+  Vector.ofFnM fun _ ↦ do
+    let varIdx ← CircuitStateM.alloc
+    return .v varIdx
+
+def test : CircuitStateM p Unit := do
+  let x ← lam
+  eq0 x
+  let y ← share (.add 1 1)
+  discard <| [1, 2, y].mapM eq0
+  eq0 4
+
+namespace CircuitState
+
+@[simp, grind =]
+lemma eval_edsl_eq0
+  (e: FixedExp p)
+  (numAlloc : ℕ)
+  (varStore)
+:
+  Edsl.CircuitState.eval (Edsl.eq0 e numAlloc).1.2 varStore numAlloc =
+  ⟨numAlloc, varStore, e.eval varStore.get? = .some 0⟩
+:= by
+  simp [
+    Clap.monads,
+    Edsl.eq0
+  ]
+
+@[simp, grind =]
+lemma eval_edsl_lam
+  (numAlloc : ℕ)
+  (varStore : Std.ExtTreeMap ℕ (ZMod p))
+:
+  Edsl.CircuitState.eval (Edsl.lam numAlloc).1.2 varStore numAlloc =
+  ⟨numAlloc + 1, varStore, True⟩
+:= by
+  simp [
+    Clap.monads,
+    Edsl.lam
+  ]
+
+@[simp, grind =]
+lemma eval_edsl_share
+  (e : FixedExp p)
+  (numAlloc : ℕ)
+  (varStore : Std.ExtTreeMap ℕ (ZMod p))
+:
+  Edsl.CircuitState.eval (Edsl.share e numAlloc).1.2 varStore numAlloc =
+  ⟨
+    numAlloc + 1,
+    varStore.insert numAlloc ((e.eval varStore.get?).getD 0),
+    (e.eval varStore.get?).isSome
+  ⟩
+:= by
+  simp [
+    Clap.monads,
+    Edsl.share
+  ]
+
+@[simp, grind =]
+lemma eval_edsl_isZero
+  (e : FixedExp p)
+  (numAlloc : ℕ)
+  (varStore : Std.ExtTreeMap ℕ (ZMod p))
+:
+  Edsl.CircuitState.eval (Edsl.isZero e numAlloc).1.2 varStore numAlloc =
+  ⟨
+    numAlloc + 1,
+    varStore.insert numAlloc (if (e.eval varStore.get?) = .some 0 then 1 else 0),
+    (e.eval varStore.get?).isSome
+  ⟩
+:= by
+  simp [
+    Clap.monads,
+    Edsl.isZero
+  ]
+
+-- TODO, trying to use this instead of the set, have, subst combo
+@[simp]
+lemma match_pair
+  (α β γ)
+  (a : Id (α × β))
+  (f : α → β → γ)
+:
+  match a with
+    | (x, y) => f x y
+  = f a.1 a.2
+:= rfl
+
+@[simp, grind =]
+lemma eval_edsl_num2bits
+  (width : ℕ)
+  (e : FixedExp p)
+  (numAlloc : ℕ)
+  (varStore : Std.ExtTreeMap ℕ (ZMod p))
+:
+  Edsl.CircuitState.eval (Edsl.num2bits width e numAlloc).1.2 varStore numAlloc =
+  ⟨
+    numAlloc + width,
+    varStore.insertMany
+      ((Vector.map (fun x => x + numAlloc) (Vector.range width)).zip
+        (num2bitsLsbPureV width ((FixedExp.eval varStore.get? e).getD 0))),
+    (e.eval varStore.get?).isSome
+  ⟩
+:= by
+  simp [
+    Clap.monads,
+    Edsl.num2bits,
+    CircuitStateM.alloc
+  ]
+  unfold StateT.pure StateT.map StateT.bind
+  simp [Clap.monads]
+  set x := @Vector.ofFnM (CircuitStateM p) _ _ _ _ _
+  have : x = ⟨x.1, x.2⟩ := rfl
+  rewrite [this]; clear this
+  subst x
+  simp [Clap.monads]
+
+end CircuitState
+
+/--
+info: (((),
+  #[Clap.CircuitusPlanus.lam, Clap.CircuitusPlanus.eq0 v0, Clap.CircuitusPlanus.share (1 + 1),
+    Clap.CircuitusPlanus.eq0 1, Clap.CircuitusPlanus.eq0 2, Clap.CircuitusPlanus.eq0 v1, Clap.CircuitusPlanus.eq0 4]),
+ 2)
+-/
+#guard_msgs in
+#eval test.run (p := 57) 0
+
+end Edsl
+
+end Clap
